  \begin{equation}\begin{gathered}\begin{aligned}
        \bar{\vFunc}_{t}({m}_{t})  & = \uFunc(\bar{\cNrm}_{t})\mathbb{C}_{t}^{T}\label{eq:vFuncPF}
        \\  & = \uFunc(\bar{c}_{t}) \MPCmin_{t}^{-1} % 20190820
        \\  & = \uFunc((\aboveMin \mNrm_{t}+\aboveMin \hEnd_{t})\MPCmin_{t}) \MPCmin_{t}^{-1} % 20190820
        \\  & = \uFunc(\aboveMin \mNrm_{t}+\aboveMin \hEnd_{t})\MPCmin_{t}^{1-\CRRA} \MPCmin_{t}^{-1} % 20190820
        \\  & = \uFunc(\aboveMin \mNrm_{t}+\aboveMin \hEnd_{t})\MPCmin_{t}^{-\CRRA}  % 20190820
      \end{aligned}\end{gathered}\end{equation}
  where the second line uses the fact demonstrated in \cite{BufferStockTheory} that $\mathbb{C}_{t}=\MPC^{-1}_{t}$. % 20190820

  This can be transformed as
  \begin{equation*}\begin{gathered}\begin{aligned}
        \bar{\vInv}_{t}  & \equiv  \left((1-\CRRA)\bar{\vFunc}_{t}\right)^{1/(1-\CRRA)}
        \\  & = \cNrm_{t}(\mathbb{C}_{t}^{T})^{1/(1-\CRRA)}
        \\  & = (\aboveMin \mNrm_{t}+\aboveMin \hEnd_{t})\MPCmin_{t}^{-\CRRA/(1-\CRRA)}   % 20190820
      \end{aligned}\end{gathered}\end{equation*}
